src/proof/kubernetes_model/update.v
@@ -1,9 +1,154 @@
 From New.proof Require Import prelude empty_ffi.
 From New.proof.kubernetes_model Require Export inv common.
+From New.proof.k8s_io.apiserver.pkg.registry Require Export rest.
 
 Section proof.
 Context `{hG: !heapGS Σ} {go_ctx: GoContext}.
 Context `{!kubernetesModelG Σ}.
+
+Lemma update_own_meta_frag_equiv_except_resource_version {γ k uid dq meta1 meta2} :
+  ObjectMetaV.equiv_except_resource_version meta1 meta2 →
+  own_meta_frag γ k uid dq meta2 -∗
+  own_meta_frag γ k uid dq meta1.
+Proof.
+  iIntros (Hmeta_eq) "Hown_meta".
+  assert (kview.mk_meta_frag k uid dq meta1 = kview.mk_meta_frag k uid dq meta2) as Hfrag_eq.
+  { rewrite /kview.mk_meta_frag /ObjectMetaV.equiv_except_resource_version in Hmeta_eq |- *.
+    rewrite Hmeta_eq. done. }
+  rewrite /own_meta_frag /kview.own_meta_frag Hfrag_eq.
+  iExact "Hown_meta".
+Qed.
+
+Lemma objectmeta_updated_set_resource_version m m' rv :
+  ObjectMetaV.updated m m' →
+  ObjectMetaV.updated m (m' <| ObjectMetaV.ResourceVersion' := rv |>).
+Proof.
+  rewrite /ObjectMetaV.updated.
+  destruct m, m'; simpl; intuition congruence.
+Qed.
+
+Lemma objectmeta_updated_set_resource_version_uid m m' rv :
+  ObjectMetaV.updated m m' →
+  ObjectMetaV.UID' (m' <| ObjectMetaV.ResourceVersion' := rv |>) =
+    ObjectMetaV.UID' m.
+Proof.
+  rewrite /ObjectMetaV.updated.
+  destruct m, m'; simpl; intuition congruence.
+Qed.
+
+Lemma valid_simple_update_updated_set_resource_version_uid m_old m_input m_updated rv :
+  ObjectMetaV.valid_simple_update m_old m_input →
+  ObjectMetaV.updated m_input m_updated →
+  ObjectMetaV.UID' (m_updated <| ObjectMetaV.ResourceVersion' := rv |>) =
+    ObjectMetaV.UID' m_old.
+Proof.
+  rewrite /ObjectMetaV.valid_simple_update /ObjectMetaV.updated.
+  destruct m_old, m_input, m_updated; simpl; intuition congruence.
+Qed.
+
+Lemma valid_simple_update_updated_set_resource_version_parent_ref m_old m_input m_updated rv :
+  ObjectMetaV.valid_simple_update m_old m_input →
+  ObjectMetaV.updated m_input m_updated →
+  meta_parent_ref m_old =
+    meta_parent_ref (m_updated <| ObjectMetaV.ResourceVersion' := rv |>).
+Proof.
+  rewrite /ObjectMetaV.valid_simple_update /ObjectMetaV.updated /meta_parent_ref.
+  destruct m_old, m_input, m_updated; simpl.
+  intros Hvalid Hupdated.
+  decompose [and] Hvalid. decompose [and] Hupdated. subst.
+  done.
+Qed.
+
+Lemma valid_simple_update_updated_set_resource_version_no_speculative_parent_reference
+    m_old m_input m_updated rv used_uid :
+  ObjectMetaV.valid_simple_update m_old m_input →
+  ObjectMetaV.updated m_input m_updated →
+  no_speculative_parent_reference m_old used_uid →
+  no_speculative_parent_reference
+    (m_updated <| ObjectMetaV.ResourceVersion' := rv |>) used_uid.
+Proof.
+  rewrite /ObjectMetaV.valid_simple_update /ObjectMetaV.updated
+          /no_speculative_parent_reference /meta_parent_ref_is /meta_parent_ref.
+  destruct m_old, m_input, m_updated; simpl.
+  intros Hvalid Hupdated Hno_spec kind name uid Hparent.
+  decompose [and] Hvalid. decompose [and] Hupdated. subst.
+  eapply Hno_spec. done.
+Qed.
+
+Lemma key_update_objectmeta_set_resource_version obj rv :
+  KObjectV.key
+    (KObjectV.update_objectmeta obj
+       ((KObjectV.objectmeta obj) <| ObjectMetaV.ResourceVersion' := rv |>)) =
+  KObjectV.key obj.
+Proof.
+  rewrite /KObjectV.key.
+  rewrite KObjectV.kind_update_objectmeta objectmeta_update_objectmeta.
+  destruct (KObjectV.objectmeta obj); done.
+Qed.
+
+Lemma valid_update_objectmeta_set_resource_version obj rv :
+  KObjectV.valid obj →
+  valid_resource_version rv →
+  KObjectV.valid
+    (KObjectV.update_objectmeta obj
+       ((KObjectV.objectmeta obj) <| ObjectMetaV.ResourceVersion' := rv |>)).
+Proof.
+  intros (Hvalid_typemeta & _ & Hvalid_meta & Hvalid_spec & Hvalid_status) Hvalid_rv.
+  split_and!.
+  - rewrite KObjectV.kind_update_objectmeta KObjectV.typemeta_update_objectmeta.
+    exact Hvalid_typemeta.
+  - rewrite objectmeta_update_objectmeta. done.
+  - rewrite objectmeta_update_objectmeta.
+    destruct (KObjectV.objectmeta obj); simpl in *; done.
+  - rewrite KObjectV.spec_update_objectmeta. done.
+  - rewrite KObjectV.status_update_objectmeta. done.
+Qed.
+
+Lemma update_tombed_uid_update_eq_used_uid_sub
+  (abs_state : gmap KKey.t KObjectV.t) (used_uid tombed_uid : gset types.UID.t)
+  key old_kobj new_kobj :
+  tombed_uid = used_uid ∖ map_to_set (C:=gset types.UID.t)
+    (λ (_ : KKey.t) (obj : KObjectV.t), ObjectMetaV.UID' (KObjectV.objectmeta obj)) abs_state →
+  abs_state !! key = Some old_kobj →
+  ObjectMetaV.UID' (KObjectV.objectmeta new_kobj) =
+    ObjectMetaV.UID' (KObjectV.objectmeta old_kobj) →
+  tombed_uid = used_uid ∖ map_to_set (C:=gset types.UID.t)
+    (λ (_ : KKey.t) (obj : KObjectV.t), ObjectMetaV.UID' (KObjectV.objectmeta obj))
+    (<[key := new_kobj]> abs_state).
+Proof.
+  intros Htombed Hlookup_abs Huid_eq.
+  set (uid := ObjectMetaV.UID' (KObjectV.objectmeta old_kobj)).
+  set (uids := λ m : gmap KKey.t KObjectV.t,
+    map_to_set (C:=gset types.UID.t)
+      (λ (_ : KKey.t) (obj : KObjectV.t), ObjectMetaV.UID' (KObjectV.objectmeta obj))
+      m).
+  assert (uids abs_state = {[uid]} ∪ uids (delete key abs_state)) as Hmap_to_set_old.
+  { rewrite /uids.
+    rewrite <- (insert_delete_id abs_state key old_kobj Hlookup_abs) at 1.
+    assert (delete key abs_state !! key = None) as Hlookup_delete.
+    { apply lookup_delete_eq. }
+    rewrite (map_to_set_insert_L
+      (λ (_ : KKey.t) (obj : KObjectV.t), ObjectMetaV.UID' (KObjectV.objectmeta obj))
+      (delete key abs_state) key old_kobj Hlookup_delete).
+    reflexivity.
+  }
+  assert (uids (<[key := new_kobj]> abs_state) = {[uid]} ∪ uids (delete key abs_state))
+    as Hmap_to_set_new.
+  { rewrite /uids.
+    rewrite <- (insert_delete_eq abs_state key new_kobj).
+    assert (delete key abs_state !! key = None) as Hlookup_delete.
+    { apply lookup_delete_eq. }
+    rewrite (map_to_set_insert_L
+      (λ (_ : KKey.t) (obj : KObjectV.t), ObjectMetaV.UID' (KObjectV.objectmeta obj))
+      (delete key abs_state) key new_kobj Hlookup_delete).
+    rewrite Huid_eq.
+    reflexivity.
+  }
+  rewrite Htombed.
+  change (used_uid ∖ uids abs_state = used_uid ∖ uids (<[key := new_kobj]> abs_state)).
+  rewrite Hmap_to_set_old Hmap_to_set_new.
+  reflexivity.
+Qed.
 
 Lemma wp_State__update_au γ l kind namespace i kobj :
   ∀ Φ,
@@ -37,6 +182,308 @@ Lemma wp_State__update_au γ l kind namespace i kobj :
               ={∅,⊤}=∗ ▷ Φ (#i', #err)%V
       )%I
     ) -∗ WP l @ (ptrT.id apimodel.State.id) @ "update" #kind #namespace #i {{ Φ }}.
-Proof. Admitted.
+Proof.
+  iIntros (Φ) "(#? & #Hkinv & Hau)". iNamed "Hau". iNamed "Hkinv".
+  wp_method_call. wp_call.
+  wp_apply wp_with_defer. iIntros (defer) "Hdefer". simpl subst. wp_auto.
+  wp_apply wp_Mutex__Lock; [done|]. iIntros "[Hown_Mutex H]". iNamedPrefix "H" "Hinv_". wp_auto.
+  wp_apply (wp_deepCopy with "[$Hdeepown_i]"). iIntros (i1) "[Hdeepown_i1 Hdeepown_i]". wp_auto.
+  iDestruct "Hdeepown_i1" as (l1) "[%Hvalid_interface Hdeepown_l]".
+  wp_apply wp_Accessor. 1: iPureIntro; done.
+  rewrite bool_decide_true //. wp_auto.
+  iPoseProof (KObjectV.deepown_l_split with "Hdeepown_l") as
+    "(Hdeepown_t_l & Hdeepown_m_l & Hdeepown_s_l & Hdeepown_st_l)".
+  wp_apply (wp_EnsureObjectNamespaceMatchesRequestNamespace with "[$Hdeepown_m_l]").
+  { iPureIntro. split. 1: done. right. done. }
+  iIntros "Hdeepown_m_l". wp_auto.
+  rewrite bool_decide_true //. wp_auto.
+  wp_apply (wp_GetName_deepown with "[$Hdeepown_m_l]"). iIntros "Hdeepown_m_l". wp_auto.
+  assert (ObjectMetaV.Name' (KObjectV.objectmeta kobj) ≠ ""%go) as Hname_not_empty.
+  { destruct Hvalid as (_ & _ & Hmeta & _). apply ObjectMetaV.valid_name_nonempty_of_valid. done. }
+  rewrite bool_decide_false //. wp_auto.
+  wp_apply (wp_map_get with "[$Hinv_Hown_phys]"). iIntros "Hinv_Hown_phys". wp_auto.
+  iDestruct (big_sepM2_dom with "Hinv_Hphys_abs_rep") as %Hdom_eq.
+  set key := {|
+    KKey.Kind' := kind;
+    KKey.Name' := ObjectMetaV.Name' (KObjectV.objectmeta kobj);
+    KKey.Namespace' := namespace
+  |}.
+  assert (key = KObjectV.key kobj) as Hkey_new.
+  { unfold key. rewrite Hkind_matches Hns_matches. destruct kobj; done. }
+  assert (namespace = (KObjectV.objectmeta kobj).(ObjectMetaV.Namespace')) as Hnamespace_new.
+  { done. }
+  destruct (bool_decide (is_Some (phys_state !! key))) eqn:Hdecide.
+  2: {
+    apply bool_decide_eq_false in Hdecide.
+    assert (phys_state !! key = None) as Hlookup_phys_none.
+    { destruct (phys_state !! key) as [i'|] eqn:Hlookup_phys; [|done].
+      exfalso. apply Hdecide. done. }
+    assert (abs_state !! key = None) as Hlookup_abs.
+    { apply not_elem_of_dom. rewrite <- Hdom_eq.
+      apply not_elem_of_dom. done. }
+    iApply fupd_wp.
+    iMod "Hau" as (key0 uid kmeta kspec) "H". iNamed "H".
+    assert (key0 = key) as ->.
+    { unfold key. rewrite Hkind_matches. rewrite Hns_matches. destruct kobj. all: done. }
+    iPoseProof (kview.own_meta_exists with "Hinv_Hown_abs Hown_meta_frag")
+      as "(%obj & %Hlookup_abs' & %Huid_obj & %Hmeta_eq & %Huid_in)".
+    assert (abs_state !! key ≠ None) as Hlookup_abs''.
+    { intros Hnone. rewrite Hlookup_abs' in Hnone. done. }
+    exfalso.
+    done.
+  }
+  assert (∃ old_i, phys_state !! key = Some old_i) as [old_i Hlookup_phys].
+  { apply bool_decide_eq_true in Hdecide. done. }
+  assert (∃ old_kobj, abs_state !! key = Some old_kobj) as [old_kobj Hlookup_abs].
+  { apply elem_of_dom. rewrite <- Hdom_eq. apply elem_of_dom. eexists. done. }
+  iDestruct (big_sepM2_delete _ phys_state abs_state key _ _ Hlookup_phys Hlookup_abs with "Hinv_Hphys_abs_rep")
+    as "(Hdeepown_old_i & Hother_rep)".
+  rewrite Hlookup_phys. wp_auto.
+  wp_apply (wp_deepCopy with "[$Hdeepown_old_i]"). iIntros (old_i1) "[Hdeepown_old_i1 Hdeepown_old_i]". wp_auto.
+  iDestruct "Hdeepown_old_i1" as (old_l1) "[%Hvalid_interface_old Hdeepown_old_l]".
+  wp_apply wp_Accessor. 1: iPureIntro; done.
+  rewrite bool_decide_true //. wp_auto.
+  iPoseProof (KObjectV.deepown_l_split with "Hdeepown_old_l") as
+    "(Hdeepown_t_old_l & Hdeepown_m_old_l & Hdeepown_s_old_l & Hdeepown_st_old_l)".
+  wp_apply (wp_GetUID_deepown with "[$Hdeepown_m_l]"). iIntros "Hdeepown_m_l". wp_auto.
+  wp_if_destruct.
+  1: {
+    exfalso.
+    destruct Hvalid as (_ & _ & Hmeta_valid & _).
+    pose proof (ObjectMetaV.valid_uid_of_valid _ Hmeta_valid) as Huid_valid.
+    pose proof (valid_uid_non_empty _ Huid_valid) as Huid_nonempty. done.
+  }
+  rewrite bool_decide_false //. wp_auto.
+  wp_apply (wp_GetUID_deepown with "[$Hdeepown_m_old_l]"). iIntros "Hdeepown_m_old_l". wp_auto.
+  wp_if_destruct.
+  2: {
+    iApply fupd_wp.
+    iMod "Hau" as (key0 uid kmeta kspec) "H". iNamed "H".
+    assert (key0 = key) as ->.
+    { rewrite Hkey_eq. unfold key. destruct kobj. all: done. }
+    iPoseProof (kview.own_meta_exists2 with "Hinv_Hown_abs Hown_meta_frag")
+      as "(%Huid_obj & %Hmeta_eq & %Huid_in)". 1: done.
+    exfalso.
+    rewrite Huid_eq in Huid_obj. symmetry in Huid_obj. done.
+  }
+  wp_apply (wp_GetResourceVersion_deepown with "[$Hdeepown_m_l]"). iIntros "Hdeepown_m_l". wp_auto.
+  wp_apply (wp_GetResourceVersion_deepown with "[$Hdeepown_m_old_l]"). iIntros "Hdeepown_m_old_l". wp_auto.
+  wp_if_destruct.
+  {
+    exfalso.
+    destruct Hvalid as (_ & Hrv_valid & _).
+    pose proof (valid_resource_version_non_empty _ Hrv_valid) as Hrv_nonempty. done.
+  }
+  rewrite bool_decide_false //. wp_auto.
+  wp_apply wp_parseResourceVersion.
+  { iPureIntro. destruct Hvalid as (_ & Hrv_valid & _). done. }
+  iIntros (ret) "_". wp_auto.
+  rewrite bool_decide_true //. wp_auto.
+  wp_apply (wp_GetResourceVersion_deepown with "[$Hdeepown_m_l]"). iIntros "Hdeepown_m_l". wp_auto.
+  wp_if_destruct.
+  2: {
+    wp_apply wp_newUpdateResourceVersionConflictError.
+    iIntros (err) "%Herr_not_nil". wp_auto.
+    iApply fupd_wp.
+    iMod "Hau" as (key0 uid kmeta kspec) "H". iNamed "H".
+    assert (key0 = key) as ->.
+    { rewrite Hkey_eq. unfold key. destruct kobj. all: done. }
+    iMod ("Hclose" $! interface.nil err kobj with "[Hown_meta_frag Hown_spec_frag]") as "HΦ".
+    { iRight. iFrame. iPureIntro. done. }
+    iModIntro.
+    iAssert (([∗ map] i; obj ∈ phys_state; abs_state, KObjectV.deepown_i i obj 1)%I)
+      with "[Hdeepown_old_i Hother_rep]" as "Hinv_Hphys_abs_rep".
+    { rewrite (big_sepM2_delete _ phys_state abs_state key _ _ Hlookup_phys Hlookup_abs).
+      iFrame. }
+    iCombineNamed "Hinv_*" as "H".
+    wp_apply (wp_Mutex__Unlock _ (kubernetes_inv γ l) with "[$Hown_Mutex H]").
+    { iNamed "H". iFrame. iFrame "#". done. }
+    iApply "HΦ".
+  }
+  set P := ObjectMetaV.valid_simple_update (KObjectV.objectmeta old_kobj) (KObjectV.objectmeta kobj) ∧
+    ObjectSpecV.valid_update (KObjectV.spec old_kobj) (KObjectV.spec kobj).
+  destruct (bool_decide(P)) eqn:Hdecide'.
+  2: {
+    iApply fupd_wp.
+    iMod "Hau" as (key0 uid kmeta kspec) "H". iNamed "H".
+    assert (key0 = key) as ->.
+    { rewrite Hkey_eq. unfold key. destruct kobj. all: done. }
+    iPoseProof (kview.own_meta_exists2 with "Hinv_Hown_abs Hown_meta_frag")
+      as "(%Huid_obj & %Hmeta_eq & %Huid_in)". 1: done.
+    iPoseProof (kview.own_spec_exists with "Hinv_Hown_abs Hown_spec_frag") as "%Hspec_found".
+    assert (KObjectV.spec old_kobj = kspec) as Hspec_eq.
+    { eapply Hspec_found; done. }
+    apply bool_decide_eq_false in Hdecide'.
+    exfalso. apply Hdecide'. unfold P.
+    split.
+    - rewrite /ObjectMetaV.valid_simple_update in Hvalid_meta_update |- *.
+      rewrite /ObjectMetaV.equiv_except_resource_version /ObjectMetaV.without_resource_version in Hmeta_eq.
+      destruct (KObjectV.objectmeta old_kobj), kmeta, (KObjectV.objectmeta kobj); simpl in *.
+      inversion Hmeta_eq; subst. tauto.
+    - rewrite Hspec_eq. done.
+  }
+  apply bool_decide_eq_true in Hdecide'.
+  unfold P in Hdecide'. destruct Hdecide' as [Hvalid_meta_old Hvalid_spec_old].
+  assert ((KObjectV.objectmeta kobj <| ObjectMetaV.Namespace' := ObjectMetaV.Namespace' (KObjectV.objectmeta kobj) |>)
+    = (KObjectV.objectmeta kobj)) as ->.
+  { destruct (KObjectV.objectmeta kobj). done. }
+  iPoseProof (KObjectV.deepown_l_restore with "[$Hdeepown_t_old_l $Hdeepown_m_old_l $Hdeepown_s_old_l $Hdeepown_st_old_l]")
+    as "Hdeepown_old_l".
+  iPoseProof (KObjectV.deepown_l_restore with "[$Hdeepown_t_l $Hdeepown_m_l $Hdeepown_s_l $Hdeepown_st_l]")
+    as "Hdeepown_l".
+  iPoseProof (kview.own_auth_valid2 key old_kobj with "Hinv_Hown_abs") as "%Hauth_old".
+  1: done.
+  destruct Hauth_old as (Hkey_old & Hvalid_old_kobj & Huid_old_in &
+    Hno_speculative_parent_reference_old & Huid_unique_old).
+  assert (KObjectV.key old_kobj = KObjectV.key kobj) as Hkey_old_new.
+  { rewrite <-Hkey_old. exact Hkey_new. }
+  wp_apply (wp_applyValidationAndDefaultingOnUpdate with "[$Hdeepown_l $Hdeepown_old_l]").
+  { iFrame "#". iPureIntro. split_and!; done. }
+  iIntros (updated_kobj) "(Hdeepown_l & Hdeepown_old_l & %Hvalid_interface_updated & %Hvalid_updated_kobj & %Hsame_key
+    & %Htypemeta_eq & %Hupdated_meta & %Hupdated_spec & %Hstatus_eq)". wp_auto.
+  rewrite bool_decide_true //. wp_auto.
+  set P' := ObjectMetaV.DeletionTimestamp' (KObjectV.objectmeta old_kobj) = None.
+  destruct (bool_decide(P')) eqn:Hdecide''.
+  2: {
+    iApply fupd_wp.
+    iMod "Hau" as (key0 uid kmeta kspec) "H". iNamed "H".
+    assert (key0 = key) as ->.
+    { rewrite Hkey_eq. symmetry. exact Hkey_new. }
+    iPoseProof (kview.own_meta_exists2 with "Hinv_Hown_abs Hown_meta_frag")
+      as "(%Huid_obj & %Hmeta_eq & %Huid_in)". 1: done.
+    apply bool_decide_eq_false in Hdecide''.
+    exfalso. apply Hdecide''. unfold P'.
+    rewrite (ObjectMetaV.equiv_except_resource_version_deletion_timestamp _ _ Hmeta_eq).
+    exact Hno_deletion_timestamp.
+  }
+  apply bool_decide_eq_true in Hdecide''. unfold P' in Hdecide''.
+  wp_apply (wp_shouldDeleteDuringUpdate with "[$Hdeepown_l $Hdeepown_old_l]").
+  { iFrame "#". iPureIntro. split_and!; done. }
+  iIntros "(Hdeepown_l & Hdeepown_old_l)". wp_auto.
+  wp_apply (wp_storageObjectDeepEqual with "[$Hdeepown_l $Hdeepown_old_l]").
+  { iPureIntro. split_and!. all: done. }
+  iIntros (v) "(Hdeepown_i1 & Hdeepown_old_i1 & %Hifv)".
+  wp_if_destruct.
+  {
+    assert (storage_object_normalize updated_kobj = storage_object_normalize old_kobj) as Hstorage_eq.
+    { apply Hifv. done. }
+    assert (ObjectMetaV.updated (KObjectV.objectmeta kobj) (KObjectV.objectmeta old_kobj))
+      as Hupdated_meta_old.
+    { eapply storage_object_normalize_objectmeta_updated; done. }
+    assert (ObjectSpecV.updated (KObjectV.spec kobj) (KObjectV.spec old_kobj))
+      as Hupdated_spec_old.
+    { assert (KObjectV.spec updated_kobj = KObjectV.spec old_kobj) as Hspec_updated_old.
+      { eapply storage_object_normalize_spec_eq. done. }
+      rewrite <-Hspec_updated_old. done. }
+    iApply fupd_wp.
+    iMod "Hau" as (key0 uid kmeta kspec) "H". iNamed "H".
+    assert (key0 = key) as ->.
+    { rewrite Hkey_eq. symmetry. exact Hkey_new. }
+    iPoseProof (kview.own_meta_exists2 with "Hinv_Hown_abs Hown_meta_frag")
+      as "(%Huid_obj & %Hmeta_eq & %Huid_in)". 1: done.
+    iPoseProof (update_own_meta_frag_equiv_except_resource_version Hmeta_eq with "Hown_meta_frag")
+      as "Hown_meta_frag".
+    iPoseProof (kview.own_spec_exists with "Hinv_Hown_abs Hown_spec_frag") as "%Hspec_found".
+    assert (KObjectV.spec old_kobj = kspec) as Hspec_eq.
+    { eapply Hspec_found; done. }
+    iMod ("Hclose" $! old_i1 interface.nil old_kobj with
+      "[Hdeepown_old_i1 Hown_meta_frag Hown_spec_frag]") as "HΦ".
+    { iLeft.
+      iSplit; first done.
+      iSplit; first done.
+      iSplit; first done.
+      iFrame "Hdeepown_old_i1 Hown_meta_frag".
+      rewrite Hspec_eq. iFrame. }
+    iModIntro.
+    iAssert (([∗ map] i; obj ∈ phys_state; abs_state, KObjectV.deepown_i i obj 1)%I)
+      with "[Hdeepown_old_i Hother_rep]" as "Hinv_Hphys_abs_rep".
+    { rewrite (big_sepM2_delete _ phys_state abs_state key _ _ Hlookup_phys Hlookup_abs).
+      iFrame. }
+    iCombineNamed "Hinv_*" as "H".
+    wp_apply (wp_Mutex__Unlock _ (kubernetes_inv γ l) with "[$Hown_Mutex H]").
+    { iNamed "H". iFrame. iFrame "#". done. }
+    iApply "HΦ".
+  }
+  wp_apply (wp_State__generateNewRVAndUpdate with "[$Hinv_Hstate_used_rv_addr $Hinv_Hown_used_rv]").
+  iIntros (rv) "(%Hlookup_phys_used_rv & %Hvalid_rv & Hinv_Hstate_used_rv_addr & Hinv_Hown_used_rv)". wp_auto.
+  iPoseProof (KObjectV.deepown_i_yields_deepown_l with "[$Hdeepown_i1]") as "Hdeepown_l". 1: done.
+  iPoseProof (KObjectV.deepown_l_split with "Hdeepown_l") as
+    "(Hdeepown_t_l & Hdeepown_m_l & Hdeepown_s_l & Hdeepown_st_l)".
+  assert (KObjectV.objectmeta_ptr l1 kobj = KObjectV.objectmeta_ptr l1 updated_kobj) as ->.
+  { destruct kobj, updated_kobj; simpl in *; simplify_eq; done. }
+  wp_apply (wp_SetResourceVersion_deepown with "[$Hdeepown_m_l]"). iIntros "Hdeepown_m_l". wp_auto.
+  wp_apply (wp_map_insert with "[$Hinv_Hown_phys]"). iIntros "Hinv_Hown_phys". wp_auto.
+  iPoseProof (KObjectV.deepown_l_merge with "[$Hdeepown_t_l $Hdeepown_m_l $Hdeepown_s_l $Hdeepown_st_l]")
+    as "Hdeepown_l".
+  set new_kmeta := (KObjectV.objectmeta updated_kobj <| ObjectMetaV.ResourceVersion' := rv |>).
+  set new_kobj := KObjectV.update_objectmeta updated_kobj new_kmeta.
+  wp_apply (wp_deepCopy i1 new_kobj with "[Hdeepown_l]").
+  { iFrame. iPureIntro. unfold new_kobj, new_kmeta. destruct updated_kobj; done. }
+  iIntros (i1') "[Hdeepown_i1' Hdeepown_i1]". wp_auto.
+  iApply fupd_wp.
+  iMod "Hau" as (key0 uid kmeta kspec) "H". iNamed "H".
+  assert (key0 = key) as ->.
+  { rewrite Hkey_eq. symmetry. exact Hkey_new. }
+  assert (kview.valid_k_uid_obj key uid new_kobj) as Hvalid_kuid_new.
+  { unfold kview.valid_k_uid_obj.
+    split_and!.
+    - unfold new_kobj, new_kmeta.
+      rewrite key_update_objectmeta_set_resource_version.
+      rewrite <- Hsame_key. done.
+    - unfold new_kobj, new_kmeta.
+      rewrite objectmeta_update_objectmeta.
+      rewrite Huid_eq.
+      symmetry. eapply objectmeta_updated_set_resource_version_uid. done.
+    - unfold new_kobj, new_kmeta.
+      eapply valid_update_objectmeta_set_resource_version; done.
+  }
+  iMod (kview.update_kobj_vs old_kobj new_kobj with
+    "[$Hinv_Hown_abs] [$Hown_meta_frag] [$Hown_spec_frag]")
+    as "(Hinv_Hown_abs & Hown_meta_frag & Hown_spec_frag)".
+  { exact Hvalid_kuid_new. }
+  { unfold new_kobj, new_kmeta.
+    rewrite objectmeta_update_objectmeta.
+    eapply valid_simple_update_updated_set_resource_version_no_speculative_parent_reference;
+      [exact Hvalid_meta_old|exact Hupdated_meta|exact Hno_speculative_parent_reference_old]. }
+  { exact Hlookup_abs. }
+  { unfold new_kobj, new_kmeta.
+    rewrite KObjectV.status_update_objectmeta. symmetry. done. }
+  iMod (cview.simple_update_vs key old_kobj new_kobj with "[$Hinv_Hown_children]")
+    as "Hinv_Hown_children".
+  { done. }
+  { unfold new_kobj, new_kmeta, obj_parent_ref.
+    rewrite objectmeta_update_objectmeta.
+    eapply valid_simple_update_updated_set_resource_version_parent_ref; done. }
+  { unfold new_kobj, new_kmeta.
+    rewrite objectmeta_update_objectmeta.
+    symmetry. eapply valid_simple_update_updated_set_resource_version_uid; done. }
+  iMod ("Hclose" $! i1' interface.nil new_kobj with
+    "[Hdeepown_i1' Hown_meta_frag Hown_spec_frag]") as "HΦ".
+  { iLeft.
+    iSplit; first done.
+    iSplit.
+    { iPureIntro. unfold new_kobj, new_kmeta.
+      rewrite objectmeta_update_objectmeta.
+      eapply objectmeta_updated_set_resource_version; done. }
+    iSplit.
+    { iPureIntro. unfold new_kobj.
+      rewrite KObjectV.spec_update_objectmeta. done. }
+    iFrame. }
+  iModIntro.
+  iAssert (([∗ map] i; obj ∈ <[key:=i1]> phys_state; <[key:=new_kobj]> abs_state,
+    KObjectV.deepown_i i obj 1)%I) with "[Hdeepown_i1 Hother_rep]" as "Hinv_Hphys_abs_rep".
+  { rewrite big_sepM2_insert_delete. iFrame. }
+  iCombineNamed "Hinv_*" as "H".
+  wp_apply (wp_Mutex__Unlock _ (kubernetes_inv γ l) with "[$Hown_Mutex H]").
+  { iNamed "H".
+    iFrame "#". iFrame. iPureIntro. split_and!.
+    all: try done.
+    eapply update_tombed_uid_update_eq_used_uid_sub; [done|done|].
+    unfold new_kobj, new_kmeta.
+    rewrite objectmeta_update_objectmeta.
+    eapply valid_simple_update_updated_set_resource_version_uid; done.
+  }
+  iApply "HΦ".
+Qed.
 
 End proof.
